Ejercicios 7.3, 7.4 y 7.5

práctica 7/Actions.v
@@ -13,8 +13,117 @@ Inductive Action :=
   | chmod : Action
 .
 
-Definition Pre := state -> Action -> Prop.
-Definition Post := state -> Action -> state -> Prop.
+Variable machine: context.
+Definition os_accessible va := ctxt_vadd_accessible machine va = true.
 
+(** READ **)
+Definition pre_read (s: state) (va: vadd) :=
+  os_accessible va /\
+  aos_activity s = running /\
+  (exists ma : madd, va_mapped_to_ma s va ma /\
+  is_RW (page_content (memory s ma))).
+
+Definition post_read (s: state) (va: vadd) (s': state) := s = s'.
+
+(** WRITE **)
+Definition pre_write (s: state) (va: vadd) (v: value) := pre_read s va.
+
+Definition post_write (s: state) (va: vadd) (v: value) (s': state) :=
+  exists ma: madd, va_mapped_to_ma s va ma /\
+  let new_page := Page (RW (Some v)) (Os (active_os s)) in
+  let new_mem := update (memory s) ma new_page in
+  mutate_memory s new_mem = s'.
+
+(** CHMOD **)
+Definition pre_chmod (s: state) :=
+  aos_activity s = waiting /\
+  let curr_os := active_os s in
+  let curr_hcall := hcall (oss s curr_os) in
+  curr_hcall = None.
+
+Definition post_chmod (s: state) (s': state) :=
+  let curr_os := active_os s in
+  let s_trusted := mutate_state s svc running in
+  let s_untrusted := mutate_state s usr running in
+  (ctxt_oss machine curr_os = true /\ s' = s_trusted) \/
+  (ctxt_oss machine curr_os = false /\ s' = s_untrusted).
+
+(* Pre and Post *)
+
+Definition Pre (s: state) (a: Action) :=
+  match a with
+    | read va    => pre_read s va
+    | write va v => pre_write s va v
+    | chmod      => pre_chmod s
+  end.
+
+Definition Post (s: state) (a: Action) (s': state) :=
+  match a with
+    | read va    => post_read s va s'
+    | write va v => post_write s va v s'
+    | chmod      => post_chmod s s'
+  end.
+
+Definition valid_state_3 (s: state) :=
+  let curr_os := active_os s in
+  let trusted := ctxt_oss machine curr_os = true in
+  let hyp_running := aos_activity s = waiting in
+  (trusted \/ hyp_running) -> aos_exec_mode s = svc.
+
+Definition valid_state_5 (s: state) :=
+  forall (os: os_ident) (pa: padd),
+  let hyp_pa_to_ma := hypervisor s os in
+  let ma_owner := fun ma => page_owned_by (memory s ma) in
+  ma_owner (hyp_pa_to_ma pa) = Os os /\
+  forall (pa': padd), hyp_pa_to_ma pa = hyp_pa_to_ma pa' -> pa = pa'.
+
+Definition valid_state_6 (s: state) :=
+  forall (page: page),
+  match page with
+    | Page (PT vm) (Os owner) =>
+        let va_owner := fun va => page_owned_by (memory s (vm va)) in
+        let accessible := ctxt_vadd_accessible machine in
+        forall (va: vadd),
+          (accessible va = true /\ va_owner va = Os owner) \/
+          (accessible va = false /\ va_owner va = Hyp)
+    | _ => True
+  end.
+
+Definition valid_state (s: state) :=
+  valid_state_3 s /\ valid_state_5 s /\ valid_state_6 s.
+
+Inductive one_step_execution (s s': state) (a: Action) :=
+  step : valid_state s -> Pre s a -> Post s a s' -> one_step_execution s s' a.
+
+Theorem execution_preserves_valid_state (a: Action) (s s': state) :
+   valid_state_3 s -> one_step_execution s s' a -> valid_state_3 s'.
+Proof.
+  unfold valid_state_3.
+  case a; intros.
+    * inversion_clear H0.
+      inversion H4.
+      rewrite <- H0 in *.
+      exact (H H1).
+    * inversion_clear H0.
+      inversion_clear H4.
+      inversion_clear H0.
+      inversion H5.
+      unfold mutate_memory in H0.
+      rewrite <- H0 in H1.
+      exact (H H1).
+    * inversion_clear H0.
+      inversion_clear H4.
+      + destruct H0.
+        rewrite -> H4.
+        reflexivity.
+      + inversion_clear H3.
+        destruct H0.
+        rewrite -> H3 in H1.
+        simpl in H1.
+        elim H1; intros.
+          - rewrite H0 in H6.
+            discriminate.
+          - discriminate.
+Qed.
 
 End Actions.
